src/Memory4.v
@@ -1,0 +1,15 @@
+Require Import bbv.Word.
+
+Section Memory.
+
+  Variable w: nat. (* bit width of addresses and memory words *)
+
+  Definition mem_access := word w -> bool.
+
+  Definition mem_contents := word w -> option (word w).
+
+  Definition memory(access: mem_access)(contents: mem_contents): Prop :=
+    forall x, access x = false <-> contents x = None.
+
+End Memory.
+
